Source/IntegrationTests/TestFiles/LitTests/LitTest/comp/rust/operators.dfy
@@ -18,7 +18,185 @@ newtype int32 = x: int  | -0x8000_0000 <= x < 0x8000_0000
 newtype int64 = x: int  | -0x8000_0000_0000_0000 <= x < 0x8000_0000_0000_0000
 newtype int128 = x: int  | -0x8000_0000_0000_0000_0000_0000_0000_0000 <= x < 0x8000_0000_0000_0000_0000_0000_0000_0000
 
-method Main() {
+method {:verify false} TestU8() {
+  var o8: uint8 := 1 as uint8;
+  var s8: uint8 := 2 as uint8;
+  var w8: uint8 := 5 as uint8;
+  var x8: uint8 := 8 as uint8;
+  var y8: uint8 := 13 as uint8;
+  var z8: uint8 := 21 as uint8;
+  var m8: uint8 := 24 as uint8;
+  var t8: uint8 := 16 as uint8;
+  if x8 + y8 == z8
+     && y8 - x8 == w8
+     && x8 as bv8 & y8 as bv8 == x8 as bv8
+     && x8 as bv8 | y8 as bv8 == y8 as bv8
+     && x8 as bv8 ^ y8 as bv8 == w8 as bv8
+     && x8 * 3 == m8
+     && x8 as bv8 >> s8 == s8 as bv8
+     && x8 as bv8 << o8 == t8 as bv8 {
+    print "operators(u8) ";
+  }
+}
+method TestI8() {
+  var o8: int8 := 1 as int8;
+  var s8: int8 := 2 as int8;
+  var w8: int8 := 5 as int8;
+  var x8: int8 := 8 as int8;
+  var y8: int8 := 13 as int8;
+  var z8: int8 := 21 as int8;
+  var m8: int8 := 24 as int8;
+  var t8: int8 := 16 as int8;
+  if x8 + y8 == z8
+     && x8 - y8 == -w8
+     && x8 * 3 == m8 {
+    print "operators(i8) ";
+  }
+}
+method {:verify false} TestU16() {
+  var o16: uint16 := 1 as uint16;
+  var s16: uint16 := 2 as uint16;
+  var w16: uint16 := 5 as uint16;
+  var x16: uint16 := 8 as uint16;
+  var y16: uint16 := 13 as uint16;
+  var z16: uint16 := 21 as uint16;
+  var m16: uint16 := 24 as uint16;
+  var t16: uint16 := 16 as uint16;
+  if x16 + y16 == z16
+     && y16 - x16 == w16
+     && x16 as bv16 & y16 as bv16 == x16 as bv16
+     && x16 as bv16 | y16 as bv16 == y16 as bv16
+     && x16 as bv16 ^ y16 as bv16 == w16 as bv16
+     && x16 * 3 == m16
+     && x16 as bv16 >> s16 as bv16 == s16 as bv16
+     && x16 as bv16 << o16 as bv16 == t16 as bv16 {
+    print "operators(u16) ";
+  }
+}
+
+method TestI16() {
+  var o16: int16 := 1 as int16;
+  var s16: int16 := 2 as int16;
+  var w16: int16 := 5 as int16;
+  var x16: int16 := 8 as int16;
+  var y16: int16 := 13 as int16;
+  var z16: int16 := 21 as int16;
+  var m16: int16 := 24 as int16;
+  var t16: int16 := 16 as int16;
+  if x16 + y16 == z16
+     && x16 - y16 == -w16
+     && x16 * 3 == m16 {
+    print "operators(i16) ";
+  }
+}
+method {:verify false} TestU32() {
+  var o32: uint32 := 1 as uint32;
+  var s32: uint32 := 2 as uint32;
+  var w32: uint32 := 5 as uint32;
+  var x32: uint32 := 8 as uint32;
+  var y32: uint32 := 13 as uint32;
+  var z32: uint32 := 21 as uint32;
+  var m32: uint32 := 24 as uint32;
+  var t32: uint32 := 16 as uint32;
+  if x32 + y32 == z32
+     && y32 - x32 == w32
+     && x32 as bv32 & y32 as bv32 == x32 as bv32
+     && x32 as bv32 | y32 as bv32 == y32 as bv32
+     && x32 as bv32 ^ y32 as bv32 == w32 as bv32
+     && x32 * 3 == m32
+     && x32 as bv32 >> s32 as bv32 == s32 as bv32
+     && x32 as bv32 << o32 as bv32 == t32 as bv32 {
+    print "operators(u32) ";
+  }
+}
+
+method TestI32() {
+  var o32: int32 := 1 as int32;
+  var s32: int32 := 2 as int32;
+  var w32: int32 := 5 as int32;
+  var x32: int32 := 8 as int32;
+  var y32: int32 := 13 as int32;
+  var z32: int32 := 21 as int32;
+  var m32: int32 := 24 as int32;
+  var t32: int32 := 16 as int32;
+  if x32 + y32 == z32
+     && x32 - y32 == -w32
+     && x32 * 3 == m32 {
+    print "operators(i32) ";
+  }
+}
+method {:verify false} TestU64() {
+  var o64: uint64 := 1 as uint64;
+  var s64: uint64 := 2 as uint64;
+  var w64: uint64 := 5 as uint64;
+  var x64: uint64 := 8 as uint64;
+  var y64: uint64 := 13 as uint64;
+  var z64: uint64 := 21 as uint64;
+  var m64: uint64 := 24 as uint64;
+  var t64: uint64 := 16 as uint64;
+  if x64 + y64 == z64
+     && y64 - x64 == w64
+     && x64 as bv64 & y64 as bv64 == x64 as bv64
+     && x64 as bv64 | y64 as bv64 == y64 as bv64
+     && x64 as bv64 ^ y64 as bv64 == w64 as bv64
+     && x64 * 3 == m64
+     && x64 as bv64 >> s64 as bv64 == s64 as bv64
+     && x64 as bv64 << o64 as bv64 == t64 as bv64 {
+    print "operators(u64) ";
+  }
+}
+method TestI64() {
+  var o64: int64 := 1 as int64;
+  var s64: int64 := 2 as int64;
+  var w64: int64 := 5 as int64;
+  var x64: int64 := 8 as int64;
+  var y64: int64 := 13 as int64;
+  var z64: int64 := 21 as int64;
+  var m64: int64 := 24 as int64;
+  var t64: int64 := 16 as int64;
+  if x64 + y64 == z64
+     && x64 - y64 == -w64
+     && x64 * 3 == m64 {
+    print "operators(i64) ";
+  }
+}
+method {:verify false} TestU128() {
+  var o128: uint128 := 1 as uint128;
+  var s128: uint128 := 2 as uint128;
+  var w128: uint128 := 5 as uint128;
+  var x128: uint128 := 8 as uint128;
+  var y128: uint128 := 13 as uint128;
+  var z128: uint128 := 21 as uint128;
+  var m128: uint128 := 24 as uint128;
+  var t128: uint128 := 16 as uint128;
+  if x128 + y128 == z128
+     && y128 - x128 == w128
+     && x128 as bv128 & y128 as bv128 == x128 as bv128
+     && x128 as bv128 | y128 as bv128 == y128 as bv128
+     && x128 as bv128 ^ y128 as bv128 == w128 as bv128
+     && x128 * 3 == m128
+     && x128 as bv128 >> s128 as bv128 == s128 as bv128
+     && x128 as bv128 << o128 as bv128 == t128 as bv128 {
+    print "operators(u128)\n";
+  }
+}
+
+method TestI128() {
+  var o128: int128 := 1 as int128;
+  var s128: int128 := 2 as int128;
+  var w128: int128 := 5 as int128;
+  var x128: int128 := 8 as int128;
+  var y128: int128 := 13 as int128;
+  var z128: int128 := 21 as int128;
+  var m128: int128 := 24 as int128;
+  var t128: int128 := 16 as int128;
+  if x128 + y128 == z128
+     && x128 - y128 == -w128
+     && x128 * 3 == m128 {
+    print "operators(i128)\n";
+  }
+}
+method {:resource_limit "200e3"}  Main() {
   var t := true;
   var f := false;
   if ((t && f) || f) ==> f {
@@ -29,111 +207,24 @@ method Main() {
   }
 
   if 2 <= 3 && 2 < 3 && 3 >= 2 && 3 > 2 && 3 != 2 && 2 == 2 {
-    print "<= < >= > != == ";
+    print "<= < >= > != ==\n";
   }
-
-  var o8: uint8 := 1 as uint8;
-  var s8: uint8 := 2 as uint8;
-  var w8: uint8 := 5 as uint8;
-  var x8: uint8 := 8 as uint8;
-  var y8: uint8 := 13 as uint8;
-  var z8: uint8 := 21 as uint8;
-  var m8: uint8 := 24 as uint8;
-  var t8: uint8 := 16 as uint8;
-  if x8 + y8 == z8
-     && y8 - x8 == z8
-     && x8 as bv8 & y8 as bv8 == x8 as bv8
-     && x8 as bv8 | y8 as bv8 == y8 as bv8
-     && x8 as bv8 ^ y8 as bv8 == w8 as bv8
-     && x8 * 3 == m8
-     && x8 as bv8 >> s8 == s8 as bv8
-     && x8 as bv8 << o8 == t8 as bv8 {
-    print "operators(u8) ";
-  }
-
+  TestU8();
+  TestU16();
+  TestU32();
+  TestU64();
+  TestU128();
+  TestI8();
+  TestI16();
+  TestI32();
+  TestI64();
+  TestI128();
   
-  var o16: uint16 := 1 as uint16;
-  var s16: uint16 := 2 as uint16;
-  var w16: uint16 := 5 as uint16;
-  var x16: uint16 := 8 as uint16;
-  var y16: uint16 := 13 as uint16;
-  var z16: uint16 := 21 as uint16;
-  var m16: uint16 := 24 as uint16;
-  var t16: uint16 := 16 as uint16;
-  if x16 + y16 == z16
-     && y16 - x16 == z16
-     && x16 as bv16 & y16 as bv16 == x16 as bv16
-     && x16 as bv16 | y16 as bv16 == y16 as bv16
-     && x16 as bv16 ^ y16 as bv16 == w16 as bv16
-     && x16 * 3 == m16
-     && x16 as bv16 >> s16 as bv16 == s16 as bv16
-     && x16 as bv16 << o16 as bv16 == t16 as bv16 {
-    print "operators(u16) ";
-  }
-  
-  var o32: uint32 := 1 as uint32;
-  var s32: uint32 := 2 as uint32;
-  var w32: uint32 := 5 as uint32;
-  var x32: uint32 := 8 as uint32;
-  var y32: uint32 := 13 as uint32;
-  var z32: uint32 := 21 as uint32;
-  var m32: uint32 := 24 as uint32;
-  var t32: uint32 := 16 as uint32;
-  if x32 + y32 == z32
-     && y32 - x32 == z32
-     && x32 as bv32 & y32 as bv32 == x32 as bv32
-     && x32 as bv32 | y32 as bv32 == y32 as bv32
-     && x32 as bv32 ^ y32 as bv32 == w32 as bv32
-     && x32 * 3 == m32
-     && x32 as bv32 >> s32 as bv32 == s32 as bv32
-     && x32 as bv32 << o32 as bv32 == t32 as bv32 {
-    print "operators(u32) ";
-  }
-
-
-  var o64: uint64 := 1 as uint64;
-  var s64: uint64 := 2 as uint64;
-  var w64: uint64 := 5 as uint64;
-  var x64: uint64 := 8 as uint64;
-  var y64: uint64 := 13 as uint64;
-  var z64: uint64 := 21 as uint64;
-  var m64: uint64 := 24 as uint64;
-  var t64: uint64 := 16 as uint64;
-  if x64 + y64 == z64
-     && y64 - x64 == z64
-     && x64 as bv64 & y64 as bv64 == x64 as bv64
-     && x64 as bv64 | y64 as bv64 == y64 as bv64
-     && x64 as bv64 ^ y64 as bv64 == w64 as bv64
-     && x64 * 3 == m64
-     && x64 as bv64 >> s64 as bv64 == s64 as bv64
-     && x64 as bv64 << o64 as bv64 == t64 as bv64 {
-    print "operators(u64)\n";
-  }
-
-  
-  var o128: uint128 := 1 as uint128;
-  var s128: uint128 := 2 as uint128;
-  var w128: uint128 := 5 as uint128;
-  var x128: uint128 := 8 as uint128;
-  var y128: uint128 := 13 as uint128;
-  var z128: uint128 := 21 as uint128;
-  var m128: uint128 := 24 as uint128;
-  var t128: uint128 := 16 as uint128;
-  if x128 + y128 == z128
-     && y128 - x128 == z128
-     && x128 as bv128 & y128 as bv128 == x128 as bv128
-     && x128 as bv128 | y128 as bv128 == y128 as bv128
-     && x128 as bv128 ^ y128 as bv128 == w128 as bv128
-     && x128 * 3 == m128
-     && x128 as bv128 >> s128 as bv128 == s128 as bv128
-     && x128 as bv128 << o128 as bv128 == t128 as bv128 {
-    print "operators(u128)\n";
-  }
-  assert {:split_here} true;
-  /*
   var a := 'a';
   var z := 'z';
-  if a < z && z > a {
+  if a < z && z > a && a <= a && a >= a && a != z && a == a
+  && !(a < a) && !(z < a) && !(z <= a) && !(a >= z)
+   {
     print "char comparison\n";
   }
   
@@ -147,9 +238,15 @@ method Main() {
   }
   var m3 := map k | 2 <= k < 4 :: k := 2*k;
   if m3 == map[3 := 6, 2 := 4] && |m3| == 2 {
-    print "comprehension equality cardinality\n";
+    print "comprehension equality cardinality ";
+  }
+  
+  if m3.Keys == {2, 3} && m3.Values == {4, 6} {
+    print ".Keys and .Values\n";
   }
 
+  // TODO: Map.Keys and Map.Values
+  /*
   var st := {1};
   if 1 in st && 2 !in st {
     print "set contains ";
@@ -160,9 +257,11 @@ method Main() {
   }
   var t3 := set k | 2 <= k < 4 :: 2*k;
   if t3 == {6, 4} && |t3| == 2 {
-    print "comprehension equality cardinality\n";
+    print "comprehension equality cardinality ";
   }
-
+  if t2 != t3 && t2 * t3 == {} {
+    print "inequality and intersection\n";
+  }
   var s1 := [1, 2];
   var s2 := s1 + [3];
   if s1 <= s2 && s1 < s2 && s1 != s2 && !(s2 <= s1)
